isabelle/Auction/Vcg/RelationProperties.thy
@@ -3,7 +3,9 @@ Auction Theory Toolbox (http://formare.github.io/auctions/)
 
 Authors:
 * Marco B. Caminati http://caminati.co.nr
+* Manfred Kerber <mnfrd.krbr@gmail.com>
 * Christoph Lange <math.semantic.web@gmail.com>
+* Colin Rowat <c.rowat@bham.ac.uk>
 
 Dually licenced under
 * Creative Commons Attribution (CC-BY) 3.0
@@ -26,11 +28,12 @@ begin
 
 section {* right-uniqueness *}
 
+(* flip is applied to pairs so that (flip (x, y)) = (y, x) *)
 lemma injflip: "inj_on flip A" by (metis flip_flip inj_on_def)
 
 lemma lm003: "card P = card (P^-1)" using assms card_image flip_conv injflip by metis
 
-lemma nn56: "card X=1 = (X={the_elem X})" 
+lemma nn56: "(card X = 1) = (X={the_elem X})" 
 by (metis One_nat_def card_Suc_eq card_empty empty_iff the_elem_eq)
 
 lemma lm007b: "trivial X = (X={} \<or> card X=1)" using 
@@ -39,10 +42,12 @@ nn56 order_refl subset_singletonD trivial_def trivial_empty by (metis(no_types))
 lemma lm004: "trivial P = trivial (P^-1)" using trivial_def subset_singletonD 
 subset_refl subset_insertI nn56 converse_inject converse_empty lm003 by metis
 
+(* The range of P restricted to X is equal to the image of X through P *)
 lemma lll85: "Range (P||X) = P``X" unfolding restrict_def by blast
-lemma lll02:  "(P || X) || Y = P || (X \<inter> Y)" 
-(* using lll00 ll52 Int_commute Int_left_commute ll41 lll01 restriction_within_domain *)
+
+lemma lll02:  "((P || X) || Y) = (P || (X \<inter> Y))" 
 unfolding restrict_def by fast
+
 lemma ll41: "Domain (R||X) = Domain R \<inter> X" using restrict_def by fastforce
 
 text {* A subrelation of a right-unique relation is right-unique. *}
@@ -53,14 +58,18 @@ lemma lll31: assumes "runiq P" shows "inj_on fst P"
 unfolding inj_on_def using assms runiq_def trivial_def trivial_imp_no_distinct 
 the_elem_eq surjective_pairing subsetI Image_singleton_iff by (metis(no_types))
 
-text {* alternative characterisation of right-uniqueness: the image of a singleton set is
-   @{const trivial}, i.e.\ an empty or singleton set. *}
+text {* alternative characterization of right-uniqueness: the image of a singleton set is
+   @{const trivial}, i.e.\ an empty or a singleton set. *}
 lemma runiq_alt: "runiq R \<longleftrightarrow> (\<forall> x . trivial (R `` {x}))" 
-unfolding runiq_def using Image_empty lm007 the_elem_eq by (metis(no_types)) 
+unfolding runiq_def using Image_empty lm007 the_elem_eq by (metis(no_types))
+ 
 text {* an alternative definition of right-uniqueness in terms of @{const eval_rel} *}
+(* Note that R `` {x} is the image of {x} under R and R ,, x gives you an element y such that R x y. Because of right-uniqueness in this case the element is determined, otherwise it may be undetermined *)
 lemma runiq_wrt_eval_rel: "runiq R = (\<forall>x . R `` {x} \<subseteq> {R ,, x})" by (metis eval_rel.simps runiq_alt trivial_def)
+
 lemma l31: assumes "runiq f" assumes "(x,y)\<in>f" shows "y=f,,x" using 
 assms runiq_wrt_eval_rel subset_singletonD Image_singleton_iff equals0D singletonE by fast
+
 lemma runiq_basic: "runiq R \<longleftrightarrow> (\<forall> x y y' . (x, y) \<in> R \<and> (x, y') \<in> R \<longrightarrow> y = y')" 
 unfolding runiq_alt lm01 by blast
 
@@ -70,7 +79,6 @@ using assms runiq_basic ImageE converse_iff subsetI by (metis(no_types))
 lemma ll68: assumes "runiq f" "y1 \<in> Range f" shows 
 "(f^-1 `` {y1} \<inter> f^-1 `` {y2} \<noteq> {}) = (f^-1``{y1}=f^-1``{y2})"
 using assms ll71 by fast
-(* ll66 by (smt Un_Int_assoc_eq) *)
 
 lemma converse_Image: 
   assumes runiq: "runiq R"
@@ -80,10 +88,10 @@ shows "(R^-1) `` R `` X \<subseteq> X" using assms by (metis converse_converse l
 lemma lll32: assumes "inj_on fst P" shows "runiq P" unfolding runiq_basic 
 using assms fst_conv inj_on_def old.prod.inject by (metis(no_types))
 
-lemma lll33: "runiq P=inj_on fst P" using lll31 lll32 by blast
-(* Another characterization of runiq, reducing to lambda-functional injectivity *)
+(* Another characterization of runiq, relating the set theoretical expression P to the injectivity of the function fst applied to P *)
+lemma lll33: "(runiq P) = (inj_on fst P)" using lll31 lll32 by blast
 
-lemma disj_Un_runiq: assumes "runiq P" "runiq Q" "Domain P \<inter> (Domain Q) = {}" shows "runiq (P Un Q)" 
+lemma disj_Un_runiq: assumes "runiq P" "runiq Q" "(Domain P) \<inter> (Domain Q) = {}" shows "runiq (P \<union> Q)" 
 using assms lll33 fst_eq_Domain lm010b by metis
 
 lemma runiq_paste1: assumes "runiq Q" "runiq (P outside Domain Q)" shows "runiq (P +* Q)"
@@ -93,15 +101,14 @@ by (metis (poly_guards_query))
 corollary runiq_paste2: assumes "runiq Q" "runiq P" shows "runiq (P +* Q)"
 using assms runiq_paste1 subrel_runiq Diff_subset Outside_def by (metis)
 
+(* Let f be a function, then its graph {(x, f x)} and all its restrictions such that P x for arbitrary P are right-unique. *)
 lemma l14: "runiq {(x,f x)| x. P x}" unfolding runiq_basic by fast
 
 lemma lm013: assumes "x \<in> Domain R" "runiq R" shows "card (R``{x})=1"
 using assms  lm007b 
 DomainE Image_singleton_iff empty_iff
 by (metis runiq_alt)
-(* lm007 nn56 runiq_def trivial_singleton 
-by (metis DomainE Image_singleton_iff empty_iff)
- Image_within_domain' *)
+
 
 text {* The image of a singleton set under a right-unique relation is a singleton set. *}
 lemma Image_runiq_eq_eval: assumes "x \<in> Domain R" "runiq R" shows "R `` {x} = {R ,, x}" 
@@ -116,13 +123,14 @@ corollary runiq_singleton_rel: "runiq {(x, y)}" using trivial_singleton lm022 by
 text {* The empty relation is right-unique *}
 lemma runiq_emptyrel: "runiq {}" using trivial_empty lm022 by blast
 
+(* characterization of right-uniqueness with  \<exists>! *)
 lemma runiq_wrt_ex1:
   "runiq R \<longleftrightarrow> (\<forall> a \<in> Domain R . \<exists>! b . (a, b) \<in> R)"
 using runiq_basic by (metis Domain.DomainI Domain.cases)
 
-text {* alternative characterisation of the fact that, if a relation @{term R} is right-unique,
+text {* alternative characterization of the fact that, if a relation @{term R} is right-unique,
   its evaluation @{term "R,,x"} on some argument @{term x} in its domain, occurs in @{term R}'s
-  range. *}
+  range. Note that we need runiq R in order to get a definite value for @{term "R,,x"} *}
 lemma eval_runiq_rel:
   assumes domain: "x \<in> Domain R"
       and runiq: "runiq R" 
@@ -136,6 +144,15 @@ lemma eval_runiq_in_Range:
       and "a \<in> Domain R"
   shows "R ,, a \<in> Range R"
 using assms by (metis Range_iff eval_runiq_rel)
+
+
+
+
+
+
+
+
+
 
 subsection {* converse *}
 
@@ -156,21 +173,16 @@ proof -
     using sup by (metis singleton_sub_trivial_uniq subset_antisym trivial_def)
 qed
 
-text {* The inverse image of the image of a set under some relation is a subset of that set,
-  if both the relation and its converse are right-unique. *}
+text {* The images of two disjoint sets under an injective function are disjoint. *}
 
 lemma disj_Domain_imp_disj_Image: assumes "Domain R \<inter> X \<inter> Y = {}" 
   assumes "runiq R"
       and "runiq (R\<inverse>)"
-  shows "R `` X \<inter> R `` Y = {}" 
+  shows "(R `` X) \<inter> (R `` Y) = {}" 
 using assms unfolding runiq_basic by blast
 
 lemma runiq_converse_paste_singleton: assumes "runiq (P^-1)" "y\<notin>(Range P)" 
 shows "runiq ((P +* {(x,y)})\<inverse>)" (is "?u (?P^-1)")
-(*using assms
-Range.RangeI Un_insert_right converse_converse converse_iff converse_subset_swap 
-insertE paste_sub_Un prod.inject runiq_basic subrel_runiq sup_bot.right_neutral
-by smt2*)
 proof -
 have "(?P) \<subseteq> P \<union> {(x,y)}" using assms by (metis paste_sub_Un)
 then have "?P^-1 \<subseteq> P^-1 \<union> ({(x,y)}^-1)" by blast
@@ -179,38 +191,6 @@ moreover have "Domain (P^-1) \<inter> Domain {(y,x)} = {}" using assms(2) by aut
 ultimately moreover have "?u (P^-1 \<union> {(y,x)})" using assms(1) by (metis disj_Un_runiq runiq_singleton_rel)
 ultimately show ?thesis by (metis subrel_runiq)
 qed
-(*by (smt2 Domain_converse Range.RangeI Un_insert_right converse_converse converse_iff converse_subset_swap insertE insert_iff paste_sub_Un prod.inject runiq_basic subrel_runiq sup_bot.right_neutral)*)
-
-
-
-
-
-
-
-
-
-
-
-
-
-
-
-
-
-
-
-
-
-
-
-
-
-
-
-
-
-
-
 
 
 
@@ -254,7 +234,7 @@ proof -
   then show ?thesis unfolding injective_def by blast
 qed
 *)
-text {* the set of all injective functions from @{term X} to @{term Y}. *}
+text {* The following is a classical definition of the set of all injective functions from @{term X} to @{term Y}. *}
 definition injections :: "'a set \<Rightarrow> 'b set \<Rightarrow> ('a \<times> 'b) set set"
 where "injections X Y = {R . Domain R = X \<and> Range R \<subseteq> Y \<and> runiq R \<and> runiq (R\<inverse>)}"
 (*
@@ -296,8 +276,7 @@ proof -
   ultimately show ?thesis unfolding sup_rels_from_def by simp
 qed
 *)
-text {* the list of all injective functions (represented as relations) from one set 
-  (represented as a list) to another set *}
+text {* The following definition is a constructive (computational) characterization of the set of all injections X Y, represented by a list. That is, we define the list of all injective functions (represented as relations) from one set (represented as a list) to another set. We formally prove the equivalence of the constructive and the classical definition in Universes.thy. *}
 fun injections_alg :: "'a list \<Rightarrow> 'b\<Colon>linorder set \<Rightarrow> ('a \<times> 'b) set list"
 where "injections_alg [] Y = [{}]" |
       "injections_alg (x # xs) Y = concat [ [ R +* {(x,y)} . y \<leftarrow> sorted_list_of_set (Y - Range R) ]
@@ -497,6 +476,8 @@ next
   finally show ?case .
 qed
 *)
-lemma Image_within_domain': fixes x R shows "x \<in> Domain R = (R `` {x} \<noteq> {})" by blast
+
+
+lemma Image_within_domain': fixes x R shows "(x \<in> Domain R) = (R `` {x} \<noteq> {})" by blast
 
 end
